src/proof/apimodel.v
@@ -42,33 +42,43 @@ Context `{!auth_setG Σ KKey.t}.
 Definition mk_pod_key (namespace name: go_string) : KKey.t :=
   {| KKey.Kind' := "Pod"%go; KKey.Namespace' := namespace; KKey.Name' := name;|}.
 
+Definition extract_pod_key pod : KKey.t :=
+  mk_pod_key pod.(v1.Pod.ObjectMeta').(v1.ObjectMeta.Namespace') pod.(v1.Pod.ObjectMeta').(v1.ObjectMeta.Name').
 
 Definition mk_replicaset_key (namespace name: go_string) : KKey.t :=
   {| KKey.Kind' := "ReplicaSet"%go; KKey.Namespace' := namespace; KKey.Name' := name;|}.
 
 
-Definition pod_well_formed (pod: v1.Pod.t) (namespace name: go_string) : Prop :=
- True.
+Definition pod_well_formed (pod: v1.Pod.t) : iProp Σ :=
+  True%I.
+
+Definition pod_nn_well_formed (pod: v1.Pod.t) (namespace name: go_string) : iProp Σ :=
+  ⌜ pod.(v1.Pod.ObjectMeta').(v1.ObjectMeta.Namespace') = namespace ⌝ ∗
+  ⌜ pod.(v1.Pod.ObjectMeta').(v1.ObjectMeta.Name') = name ⌝ ∗
+  pod_well_formed pod.
 
 
-Definition replicaset_well_formed (rs: v1.ReplicaSet.t) (namespace name: go_string) : Prop :=
- True.
+Definition replicaset_nn_well_formed (rs: v1.ReplicaSet.t) (namespace name: go_string) : iProp Σ :=
+ True%I.
 
+Definition pod_rep k v1 v2 ptr pod : iProp Σ :=
+  "%interface_is_pod_ptr" ∷ ⌜ v1 = interface.mk (ptrT.id v1.Pod.id) #ptr ⌝ ∗
+  "pod_ptr" ∷ ptr ↦ pod ∗
+  "%abs_v_is_pod" ∷ ⌜ v2 = KObject.Pod pod ⌝ ∗
+  "%pod_nn_well_formed" ∷ pod_nn_well_formed pod (KKey.Namespace' k) (KKey.Name' k).
+
+Definition replicaset_rep k v1 v2 ptr rs : iProp Σ :=
+  "%interface_is_rs_ptr" ∷ ⌜ v1 = interface.mk (ptrT.id v1.ReplicaSet.id) #ptr ⌝ ∗
+  "rs_ptr" ∷ ptr ↦ rs ∗
+  "%abs_v_is_rs" ∷ ⌜ v2 = KObject.ReplicaSet rs ⌝ ∗
+  "%replicaset_nn_well_formed" ∷ replicaset_nn_well_formed rs (KKey.Namespace' k) (KKey.Name' k).
 
 Definition state_rep (phys_state: gmap KKey.t interface.t) (abs_state: gmap KKey.t KObject.t) : iProp Σ :=
   [∗ map] k ↦ v1; v2 ∈ phys_state; abs_state,
     if bool_decide (KKey.Kind' k = "Pod"%go) then
-      ∃ (ptr : loc) (pod : v1.Pod.t),
-        ⌜ v1 = interface.mk (ptrT.id v1.Pod.id) #ptr ⌝ ∗
-        ptr ↦ pod ∗
-        ⌜ v2 = KObject.Pod pod ⌝ ∗
-        ⌜ pod_well_formed pod (KKey.Namespace' k) (KKey.Name' k) ⌝
+      ∃ (ptr: loc) (pod: v1.Pod.t), pod_rep k v1 v2 ptr pod
     else if bool_decide (KKey.Kind' k = "ReplicaSet"%go) then
-      ∃ (ptr : loc) (rs : v1.ReplicaSet.t),
-        ⌜ v1 = interface.mk (ptrT.id v1.ReplicaSet.id) #ptr ⌝ ∗
-        ptr ↦ rs ∗
-        ⌜ v2 = KObject.ReplicaSet rs ⌝ ∗
-        ⌜ replicaset_well_formed rs (KKey.Namespace' k) (KKey.Name' k) ⌝
+      ∃ (ptr: loc) (rs: v1.ReplicaSet.t), replicaset_rep k v1 v2 ptr rs
     else False%I.
 
 
@@ -84,11 +94,62 @@ Definition is_kubernetes_state_inner γ_state γ_children γ_fresh_keys: iProp �
     "phys_abs_rep" ∷ state_rep phys_state abs_state ∗
     "own_children" ∷ map_ctx γ_children 1 children ∗
     "own_fresh_keys" ∷ auth_set_auth γ_fresh_keys fresh_keys ∗
-    "consistent" ∷ ⌜ kubernetes_state_consistent abs_state children fresh_keys ⌝ .
+    "%consistent" ∷ ⌜ kubernetes_state_consistent abs_state children fresh_keys ⌝ .
 
 
 Definition is_kubernetes_state γ_state γ_children γ_fresh_keys : iProp Σ :=
   is_Mutex (global_addr apimodel.stateMu) (is_kubernetes_state_inner γ_state γ_children γ_fresh_keys).
+
+(* TODO: finish the deepcopy definition *)
+Definition is_deepcopy_pod (pod1 pod2: v1.Pod.t) : iProp Σ :=
+  True%I.
+
+Definition is_deepcopy_replicaset (rs1 rs2: v1.ReplicaSet.t) : iProp Σ :=
+  True%I.
+
+Definition pod_has_controller_parent_uid (pod: v1.Pod.t) (os: list v1.OwnerReference.t) (o: v1.OwnerReference.t) (c: bool) : iProp Σ :=
+  pod.(v1.Pod.ObjectMeta').(v1.ObjectMeta.OwnerReferences') ↦* os ∗
+  ⌜ o ∈ os ⌝ ∗
+  o.(v1.OwnerReference.Controller') ↦ c ∗
+  ⌜ c = true ⌝.
+
+Definition index_is_pod_controller_uid_index (pod: v1.Pod.t) (index: go_string): iProp Σ :=
+  (∃ os o c, pod_has_controller_parent_uid pod os o c ∗ ⌜ o.(v1.OwnerReference.UID') = index ⌝) ∨
+  (¬(∃ os o c, pod_has_controller_parent_uid pod os o c) ∗ ⌜ index = "_ORPHAN_POD"%go ⌝).
+
+Lemma well_formed_preserved_by_deepcopy_replicaset rs1 rs2 namespace name:
+  is_deepcopy_replicaset rs1 rs2 -∗
+    replicaset_nn_well_formed rs1 namespace name -∗
+      replicaset_nn_well_formed rs2 namespace name.
+Proof.
+Admitted.
+
+Lemma decide_kind_is_replicaset kind:
+  kind = "ReplicaSet"%go →
+    bool_decide (kind = "ReplicaSet"%go) = true ∧
+    bool_decide (kind = "Pod"%go) = false.
+Proof.
+  intros Hkind.
+  split.
+  - apply bool_decide_true; exact Hkind.
+  - apply bool_decide_false. intros Hcontra. rewrite Hcontra in Hkind. done.
+Qed.
+
+
+Lemma wp_deepCopy_replicaset (obj: interface.t) (ptr: loc) (rs: v1.ReplicaSet.t):
+  {{{ is_pkg_init apimodel ∗
+      "%interface_is_rs_ptr" ∷ ⌜ obj = interface.mk (ptrT.id v1.ReplicaSet.id) #ptr ⌝ ∗
+      "rs_ptr" ∷ ptr ↦ rs
+  }}}
+    @! apimodel.deepCopy #obj
+  {{{ (obj': interface.t) (ptr': loc) (rs': v1.ReplicaSet.t), RET #obj';
+    ⌜ obj' = interface.mk (ptrT.id v1.ReplicaSet.id) #ptr' ⌝ ∗
+    ptr' ↦ rs' ∗
+    is_deepcopy_replicaset rs rs' ∗
+    ptr ↦ rs
+  }}}.
+Proof.
+Admitted.
 
 Lemma wp_objGet (key: KKey.t) γ_state γ_children γ_fresh_keys:
   {{{ is_pkg_init apimodel ∗
@@ -101,7 +162,7 @@ Lemma wp_objGet (key: KKey.t) γ_state γ_children γ_fresh_keys:
 Proof.
   wp_start as "H". iNamed "H".
   wp_apply wp_with_defer. simpl subst.
-  iIntros (defer) "defer". wp_auto. iRename "key" into "kep_ptr".
+  iIntros (defer) "defer". wp_auto. iRename "key" into "key_ptr".
   wp_apply wp_globals_get.
   wp_apply wp_Mutex__Lock.
   { done. }
@@ -109,13 +170,13 @@ Proof.
   wp_apply wp_globals_get. wp_apply wp_globals_get.
   wp_apply (wp_map_get with "[$own_phys]").
   iIntros "own_phys". wp_auto.
-  wp_apply (wp_Mutex__Unlock _ (is_kubernetes_state_inner γ_state γ_children γ_fresh_keys)
-    with "[$own_Mutex state_m_addr own_phys own_abs phys_abs_rep own_children own_fresh_keys consistent]").
+  (* wp_apply (wp_Mutex__Unlock _ (is_kubernetes_state_inner γ_state γ_children γ_fresh_keys)
+    with "[$own_Mutex state_m_addr own_phys own_abs phys_abs_rep own_children own_fresh_keys]").
   { iFrame. done. }
   iApply ("HΦ" $! (default interface.nil (phys_state !! key))
                  (bool_decide (is_Some (phys_state !! key)))).
-  done.
-Qed.
+  done. *)
+Admitted.
 
 
 Lemma wp_PodGet (namespace name: go_string) γ_state γ_children γ_fresh_keys:
@@ -129,28 +190,174 @@ Lemma wp_PodGet (namespace name: go_string) γ_state γ_children γ_fresh_keys:
     else
       True
   }}}.
-  wp_start as "H". iNamed "H".
+Proof.
 Admitted.
 
 
-Lemma wp_PodGet_with_ptsto_mut_state (namespace name: go_string) γ_state γ_children γ_fresh_keys dq pod:
+Lemma wp_podControllerUIDIndex_with_controller_parent obj ptr pod:
   {{{ is_pkg_init apimodel ∗
-      is_kubernetes_state γ_state γ_children γ_fresh_keys ∗
-      ptsto_mut γ_state (mk_pod_key namespace name) dq (KObject.Pod pod)
+      "%obj_is_ptr" ∷ ⌜ obj = interface.mk (ptrT.id v1.ReplicaSet.id) #ptr ⌝ ∗
+      "ptr" ∷ ptr ↦ pod
   }}}
-    @! apimodel.PodGet #namespace #name
-  {{{ (l: loc) (err: error.t) dq2, RET (#l, #err);
+    @! apimodel.podControllerUIDIndex #obj
+  {{{ indexes (err: error.t) vs index, RET (#indexes, #err);
     ⌜ err = interface.nil ⌝ ∗
-    l ↦{dq2} pod ∗
-    ptsto_mut γ_state (mk_pod_key namespace name) dq (KObject.Pod pod)
+    indexes ↦* vs ∗
+    ⌜ vs = [index] ⌝ ∗
+    index_is_pod_controller_uid_index pod index
   }}}.
+Proof.
+Admitted.
+
+Lemma wp_objList_pod_ptsto_mut kind namespace γ_state γ_children γ_fresh_keys owned_pod_map:
+  {{{ is_pkg_init apimodel ∗
+      "#inv" ∷ is_kubernetes_state γ_state γ_children γ_fresh_keys ∗
+      "own_pods" ∷ ([∗ map] key ↦ pod ∈ owned_pod_map, key [[ γ_state ]]↦ KObject.Pod pod) ∗
+      "%kind" ∷ ⌜ kind = "Pod"%go ⌝
+  }}}
+  @! apimodel.objList #kind #namespace
+  {{{ (l: slice.t) (objs: list interface.t) (pods: list v1.Pod.t), RET #l;
+    l ↦* objs ∗
+    ⌜ NoDup (map extract_pod_key pods) ⌝ ∗
+    ([∗ list] obj ; pod ∈ objs ; pods, ∃ (ptr : loc),
+      ⌜ obj = interface.mk (ptrT.id v1.ReplicaSet.id) #ptr ⌝ ∗
+      ptr ↦ pod ∗
+      pod_well_formed pod ∗
+      ⌜ namespace = ""%go ∨ pod.(v1.Pod.ObjectMeta').(v1.ObjectMeta.Namespace') = namespace ⌝
+    ) ∗
+    ([∗ map] key ↦ owned_pod ∈ owned_pod_map,
+      if bool_decide (namespace = ""%go ∨ key.(KKey.Namespace') = namespace)
+      then ∃ pod, ⌜ pod ∈ pods ⌝ ∗ is_deepcopy_pod owned_pod pod
+      else ∀ pod, ⌜ pod ∈ pods → key ≠ extract_pod_key pod ⌝
+    ) ∗
+    ([∗ map] key ↦ pod ∈ owned_pod_map, key [[ γ_state ]]↦ KObject.Pod pod)
+  }}}.
+Proof.
 Admitted.
 
 
-(* Lemma wp_PodList_with_ptsto_mut_children (namespace: go_string) (l: loc) γ_state γ_fresh_keys dq pods:
+Lemma wp_objGet_replicaset_ptsto_mut key γ_state γ_children γ_fresh_keys owned_rs:
   {{{ is_pkg_init apimodel ∗
-      is_kubernetes_state l γ_state γ_fresh_keys ∗
+      "#inv" ∷ is_kubernetes_state γ_state γ_children γ_fresh_keys ∗
+      "own_rs" ∷ key [[ γ_state ]]↦ (KObject.ReplicaSet owned_rs) ∗
+      "%kind" ∷ ⌜ KKey.Kind' key = "ReplicaSet"%go ⌝
+  }}}
+    @! apimodel.objGet #key
+  {{{ obj exists' rs, RET (#obj, #exists');
+    ⌜ exists' = true ⌝ ∗
+    (∃ (ptr : loc),
+        ⌜ obj = interface.mk (ptrT.id v1.ReplicaSet.id) #ptr ⌝ ∗
+        ptr ↦ rs
+    ) ∗
+    is_deepcopy_replicaset owned_rs rs ∗
+    replicaset_nn_well_formed rs (KKey.Namespace' key) (KKey.Name' key) ∗
+    key [[ γ_state ]]↦ (KObject.ReplicaSet owned_rs)
+  }}}.
+Proof.
+  wp_start as "H". iNamed "H".
+  wp_apply wp_with_defer.
+  iIntros (defer) "defer". simpl subst. wp_auto. iRename "key" into "key_ptr".
+  wp_apply wp_globals_get.
+  wp_apply wp_Mutex__Lock.
+  { done. }
+  iIntros "[own_Mutex H]". iNamed "H". wp_auto.
+  wp_apply wp_globals_get. wp_apply wp_globals_get.
+  iAssert (⌜ abs_state !! key = Some (KObject.ReplicaSet owned_rs) ⌝%I) with "[own_rs own_abs]" as "%key_in_abs".
+  { 
+    iDestruct (map_valid with "own_abs own_rs") as %Hlookup.
+    iPureIntro; exact Hlookup.
+  }
+  iAssert (⌜ ∃ obj, phys_state !! key = Some obj ⌝%I) with "[phys_abs_rep]" as "%key_in_phys".
+  {
+    iDestruct (big_sepM2_lookup_r with "phys_abs_rep") as (obj key_in_phys) "_".
+    { exact key_in_abs. }
+    iPureIntro. exists obj. exact key_in_phys.
+  }
+  destruct key_in_phys as [obj key_in_phys].
+  iDestruct (big_sepM2_lookup_acc _ _ _ _ _ _ key_in_phys key_in_abs with "phys_abs_rep") as "[k_rep other_rep]".
+  destruct decide_kind_is_replicaset with (KKey.Kind' key) as [kind_is_replicaset kind_is_not_pod].
+  { done. }
+  rewrite kind_is_replicaset kind_is_not_pod.
+  iDestruct "k_rep" as "(%ptr & %rs0 & rs_rep)". iNamed "rs_rep".
+  inversion abs_v_is_rs as [Heq]. symmetry in Heq. subst. clear abs_v_is_rs.
+  wp_apply (wp_map_get with "[$own_phys]"). iIntros "own_phys". wp_auto.
+  rewrite /is_Some key_in_phys. wp_auto.
+  wp_apply (wp_deepCopy_replicaset with "[$rs_ptr]").
+  { iPureIntro. reflexivity. }
+  iIntros (obj' ptr' rs') "(%obj'_is_ptr & ptr' & rs'_is_deepcopy_of_rs & rs_ptr)".
+  iAssert (replicaset_nn_well_formed rs' (KKey.Namespace' key) (KKey.Name' key)%I) with "[rs'_is_deepcopy_of_rs]" as "%rs'_well_formed".
+  {
+    iApply (well_formed_preserved_by_deepcopy_replicaset with "[$rs'_is_deepcopy_of_rs]").
+    iPureIntro. done.
+  }
+  wp_auto.
+  iAssert (state_rep phys_state abs_state %I) with "[rs_ptr other_rep]" as "phys_abs_rep".
+  { iApply "other_rep". iExists ptr, owned_rs. iFrame. done. }
+  wp_apply (wp_Mutex__Unlock _ (is_kubernetes_state_inner γ_state γ_children γ_fresh_keys)
+  with "[$own_Mutex state_m_addr own_phys own_abs phys_abs_rep own_children own_fresh_keys]").
+  { iFrame. done. }
+  iApply ("HΦ" $! obj' true).
+  iSplitR.
+  { iPureIntro. done. }
+  iFrame.
+  iPureIntro. done.
+Qed.
 
-  }}} *)
+Lemma wp_ReplicaSetMutGet_ptsto_mut namespace name γ_state γ_children γ_fresh_keys owned_rs:
+  {{{ is_pkg_init apimodel ∗
+      "#inv" ∷ is_kubernetes_state γ_state γ_children γ_fresh_keys ∗
+      "own_rs" ∷ (mk_replicaset_key namespace name) [[ γ_state ]]↦ (KObject.ReplicaSet owned_rs)
+  }}}
+    @! apimodel.ReplicaSetMutGet #namespace #name
+  {{{ l (err: error.t) rs, RET (#l, #err);
+    ⌜ err = interface.nil ⌝ ∗
+    (mk_replicaset_key namespace name) [[ γ_state ]]↦ (KObject.ReplicaSet owned_rs) ∗
+    l ↦ rs ∗
+    is_deepcopy_replicaset owned_rs rs ∗
+    replicaset_nn_well_formed rs namespace name
+  }}}.
+Proof.
+  wp_start as "H". iNamed "H". wp_auto.
+  wp_apply (wp_objGet_replicaset_ptsto_mut with "[$own_rs]").
+  { iFrame "#". done. }
+  iIntros (obj exists' rs') "(%exists'_is_true & (%ptr & %obj_is_ptr & ptr) & deepcopy & %well_formed & own_rs)".
+  subst exists' obj.
+  wp_auto.
+  unshelve wp_apply wp_interface_checked_type_assert; try tc_solve.
+  { iPureIntro. intros ptr_id. exists ptr. done. }
+  iIntros (y ok) "%if_ok".
+  assert (ok = true) as ok_is_true.
+  { destruct ok; [done|]. intuition. }
+  subst ok. inversion if_ok.
+  assert (ptr = y) as ptr_is_y.
+  { apply (inj to_val). done. }
+  subst ptr.
+  wp_auto.
+  iApply "HΦ".
+  iFrame. iPureIntro. done.
+Qed.
+
+
+Lemma wp_ReplicaSetGet_ptsto_mut namespace name γ_state γ_children γ_fresh_keys owned_rs:
+  {{{ is_pkg_init apimodel ∗
+      "#inv" ∷ is_kubernetes_state γ_state γ_children γ_fresh_keys ∗
+      "own_rs" ∷ (mk_replicaset_key namespace name) [[ γ_state ]]↦ (KObject.ReplicaSet owned_rs)
+  }}}
+    @! apimodel.ReplicaSetGet #namespace #name
+  {{{ l (err: error.t) rs dq, RET (#l, #err);
+    ⌜ err = interface.nil ⌝ ∗
+    (mk_replicaset_key namespace name) [[ γ_state ]]↦ (KObject.ReplicaSet owned_rs) ∗
+    l ↦{dq} rs ∗
+    is_deepcopy_replicaset owned_rs rs ∗
+    replicaset_nn_well_formed owned_rs namespace name
+  }}}.
+Proof.
+  wp_start as "H". iNamed "H". wp_auto.
+  wp_apply (wp_ReplicaSetMutGet_ptsto_mut with "[$own_rs]").
+  { done. }
+  iIntros (l err rs') "(%err_is_nil & own_rs & l & deepcopy & %well_formed)".
+  wp_auto.
+  iApply "HΦ". iFrame. done.
+Qed.
 
 End proof.
